trying to sketch what a dependent representation
- The main annoyingness is having to know when you
  have to know the type expected from the query
  operation.
  It turns out that you'll probably always know this, but
  just the fact that you have to provide the information
  could be difficult.
  - At the very least the question is whether there is
    any performance penalty to it.
*** I need to know the answer for my thesis.

theories/ExprI.v
@@ -3,6 +3,7 @@ Require Import Relations.Relation_Definitions.
 Require Import ExtLib.Tactics.
 Require Import ExtLib.Data.HList.
 Require Import ExtLib.Data.Option.
+Require Import ExtLib.Data.Eq.
 Require Import MirrorCore.TypesI.
 Require Import MirrorCore.EnvI.
 
@@ -13,83 +14,198 @@ Section Expr.
   Variable typ : Type.
   Variable RType_typ : RType typ.
 
-  Variable expr : Type.
+  Variable expr : tenv typ -> tenv typ -> typ -> Type.
 
-  Definition ResType (us vs : tenv typ) (T : Type) : Type :=    option (hlist (typD nil) us -> hlist (typD nil) vs -> T).
+  Definition OpenT (us vs : tenv typ) (T : Type) : Type :=
+    hlist (typD nil) us -> hlist (typD nil) vs -> T.
+
+  Definition ResType (us vs : tenv typ) (T : Type) : Type :=
+    option (OpenT us vs T).
+
+  Lemma eq_ResType_eq_us
+  : forall tus tus' tvs T (pf : tus = tus') v,
+      match pf in _ = x return ResType x tvs T with
+        | eq_refl => v
+      end =
+      match v with
+        | None => None
+        | Some res => Some
+          match pf in _ = x return OpenT x tvs T with
+            | eq_refl => res
+          end
+      end.
+  Proof.
+    destruct pf; destruct v; reflexivity.
+  Qed.
+  Lemma eq_ResType_eq_vs
+  : forall tus tvs tvs' T (pf : tvs = tvs') v,
+      match pf in _ = x return ResType tus x T with
+        | eq_refl => v
+      end =
+      match v with
+        | None => None
+        | Some res => Some
+          match pf in _ = x return OpenT tus x T with
+            | eq_refl => res
+          end
+      end.
+  Proof.
+    destruct pf; destruct v; reflexivity.
+  Qed.
+  Lemma eq_OpenT_eq_us
+  : forall tus tus' tvs T (pf : tus = tus') v us vs,
+      match pf in _ = x return OpenT x tvs T with
+        | eq_refl => v
+      end us vs =
+      v match eq_sym pf in _ = x return hlist (typD nil) x with
+          | eq_refl => us
+        end vs.
+  Proof. destruct pf. reflexivity. Qed.
+  Lemma eq_OpenT_eq_vs
+  : forall tus tvs tvs' T (pf : tvs = tvs') v us vs,
+      match pf in _ = x return OpenT tus x T with
+        | eq_refl => v
+      end us vs =
+      v us match eq_sym pf in _ = x return hlist (typD nil) x with
+             | eq_refl => vs
+           end.
+  Proof. destruct pf. reflexivity. Qed.
+  Hint Rewrite eq_ResType_eq_us eq_ResType_eq_vs : eq_rw.
+  Hint Rewrite eq_OpenT_eq_us eq_OpenT_eq_vs : eq_rw.
 
   (** NOTE:
-   ** - Right now this is intensionally weak, but it should probably include
-   **   a few more operations given that it is already specialized for both
-   **   [UVar] and [Var].
    ** - An alternative is to generalize it monadically and eliminate the
    **   specialized variable environments.
    ** - Note that this interface does not support GADTs
    **)
   Class Expr : Type :=
-  { exprD' : forall (us vs : tenv typ),
-               expr -> forall (t : typ),
-                         ResType us vs (typD nil t)
+  { exprD' : forall (tus tvs : tenv typ) (t : typ),
+               expr tus tvs t -> ResType tus tvs (typD nil t)
+(*
   ; Expr_acc : relation expr
   ; wf_Expr_acc : well_founded Expr_acc
-  ; mentionsU : nat -> expr -> bool
-  ; mentionsV : nat -> expr -> bool
+*)
+  ; mentionsU
+    : forall (tus tvs : tenv typ) (t : typ), nat -> expr tus tvs t -> bool
+  ; mentionsV
+    : forall (tus tvs : tenv typ) (t : typ), nat -> expr tus tvs t -> bool
+  ; weaken
+    : forall (tus tvs : tenv typ ) (t : typ)
+             (tus' tvs' : tenv typ),
+        expr tus tvs t -> expr (tus ++ tus') (tvs ++ tvs') t
+  ; strengthen
+    : forall (tus tvs : tenv typ) (t : typ)
+             (tus' tvs' : tenv typ),
+        expr (tus ++ tus') (tvs ++ tvs') t -> option (expr tus tvs t)
   }.
+  Arguments exprD' {Expr} tus tvs t e : rename.
+
+  (* NOTE: these could all be more efficient... *)
+  Definition strengthenU (E : Expr) (tus tvs : tenv typ) t (tus' : tenv typ)
+             (e : expr (tus ++ tus') tvs t)
+  : option (expr tus tvs t) :=
+    let e :=
+        match eq_sym (app_nil_r_trans tvs) in _ = T
+              return expr (tus ++ tus') T t
+        with
+          | eq_refl => e
+        end
+    in
+    @strengthen E tus tvs t tus' nil e.
+
+  Definition strengthenV (E : Expr) (tus tvs : tenv typ) t (tvs' : tenv typ)
+             (e : expr tus (tvs ++ tvs') t)
+  : option (expr tus tvs t) :=
+    let e :=
+        match eq_sym (app_nil_r_trans tus) in _ = T
+              return expr T (tvs ++ tvs') t
+        with
+          | eq_refl => e
+        end
+    in
+    @strengthen E tus tvs t nil tvs' e.
+
+  Definition weakenU (E : Expr) (tus tvs : tenv typ) t (tus' : tenv typ)
+             (e : expr tus tvs t)
+  : expr (tus ++ tus') tvs t :=
+    match app_nil_r_trans tvs in _ = T
+          return expr (tus ++ tus') T t
+    with
+      | eq_refl => (@weaken E tus tvs t tus' nil e)
+    end.
+
+  Definition weakenV (E : Expr) (tus tvs : tenv typ) t (tvs' : tenv typ)
+             (e : expr tus tvs t)
+  : expr tus (tvs ++ tvs') t :=
+    match app_nil_r_trans tus in _ = T
+          return expr T (tvs ++ tvs') t
+    with
+      | eq_refl => (@weaken E tus tvs t nil tvs' e)
+    end.
 
   Theorem exprD'_conv (E : Expr)
-  : forall tus tus' tvs tvs' e t
+  : forall tus tus' tvs tvs' t (e : expr tus tvs t)
       (pfu : tus' = tus) (pfv : tvs' = tvs),
-      exprD' tus tvs e t = match pfu in _ = tus'
+      exprD' tus tvs t e = match pfu in _ = tus'
                                , pfv in _ = tvs'
-                                 return ResType tus' tvs' (typD nil t)
+                                 return expr tus' tvs' t -> ResType tus' tvs' (typD nil t)
                            with
-                             | eq_refl , eq_refl => exprD' tus' tvs' e t
-                           end.
+                             | eq_refl , eq_refl =>
+                               exprD' tus' tvs' t
+                           end e.
   Proof.
     destruct pfu. destruct pfv. reflexivity.
-  Qed.
+  Defined.
 
-  Definition Safe_expr {E : Expr} (tus tvs : tenv typ) (e : expr) (t : typ)
+  Definition Safe_expr {E : Expr} (tus tvs : tenv typ) (t : typ)
+             (e : expr tus tvs t)
   : Prop :=
-    exists val, exprD' tus tvs e t = Some val.
+    exists val, exprD' tus tvs t e = Some val.
+  Arguments Safe_expr {Expr} tus tvs t e : rename.
 
   Theorem Safe_expr_exprD {E : Expr}
-  : forall us vs e t,
-      Safe_expr us vs e t <->
-      exists val, exprD' us vs e t = Some val.
+  : forall tus tvs t (e : expr tus tvs t),
+      Safe_expr tus tvs t e <->
+      exists val, exprD' tus tvs t e = Some val.
   Proof. reflexivity. Qed.
 
-  Definition exprD {E : Expr} (uvar_env var_env : env nil) (e : expr) (t : typ)
+(*
+  Definition exprD {E : Expr} (uvar_env var_env : env nil) (t : typ)
+             (e : expr)
   : option (typD nil t) :=
     let (tus,us) := split_env uvar_env in
     let (tvs,vs) := split_env var_env in
-    match exprD' tus tvs e t with
+    match exprD' tus tvs t e with
       | None => None
       | Some f => Some (f us vs)
     end.
+*)
 
   Class ExprOk (E : Expr) : Type :=
   { exprD'_weaken
-    : forall tus tvs e t val,
-        exprD' tus tvs e t = Some val ->
+    : forall tus tvs t (e:expr tus tvs t) val,
+        exprD' tus tvs t e = Some val ->
         forall tus' tvs',
         exists val',
-             exprD' (tus ++ tus') (tvs ++ tvs') e t = Some val'
+             exprD' (tus ++ tus') (tvs ++ tvs') t (weaken tus' tvs' e) = Some val'
           /\ forall us vs us' vs',
                val us vs = val' (hlist_app us us') (hlist_app vs vs')
   ; exprD'_strengthenU_single
-    : forall tus tvs e t t' val,
+    : forall tus tvs t t' (e : expr (tus ++ t :: nil) tvs t') val,
       mentionsU (length tus) e = false ->
-      exprD' (tus ++ t :: nil) tvs e t' = Some val ->
-      exists val',
-        exprD' tus tvs e t' = Some val' /\
+      exprD' (tus ++ t :: nil) tvs t' e = Some val ->
+      exists val' (e' : expr tus tvs t'),
+        @strengthenU E tus tvs t' (t :: nil) e = Some e' /\
+        exprD' tus tvs t' e' = Some val' /\
         forall us vs u,
           val (hlist_app us (Hcons u Hnil)) vs = val' us vs
   ; exprD'_strengthenV_single
-    : forall tus tvs e t t' val,
+    : forall tus tvs t t' (e:expr tus (tvs ++ t :: nil) t') val,
       mentionsV (length tvs) e = false ->
-      exprD' tus (tvs ++ t :: nil) e t' = Some val ->
-      exists val',
-        exprD' tus tvs e t' = Some val' /\
+      exprD' tus (tvs ++ t :: nil) t' e = Some val ->
+      exists val' (e' : expr tus tvs t'),
+        @strengthenV E tus tvs t' (t :: nil) e = Some e' /\
+        exprD' tus tvs t' e' = Some val' /\
         forall us vs u,
           val us (hlist_app vs (Hcons u Hnil)) = val' us vs
   }.
@@ -97,10 +213,10 @@ Section Expr.
   Context {Expr_expr : Expr}.
 
   Lemma exprD'_weakenU (EOk : ExprOk Expr_expr)
-  : forall tus tus' tvs e t val,
-      exprD' tus tvs e t = Some val ->
+  : forall tus tus' tvs t e val,
+      exprD' tus tvs t e = Some val ->
       exists val',
-        exprD' (tus ++ tus') tvs e t = Some val'
+        exprD' (tus ++ tus') tvs t (weakenU _ tus' e) = Some val'
         /\ forall us vs us',
              val us vs = val' (hlist_app us us') vs.
   Proof.
@@ -111,29 +227,20 @@ Section Expr.
     instantiate (1 := app_nil_r_trans _).
     instantiate (1 := eq_refl).
     simpl.
+    unfold weakenU.
+    autorewrite with eq_rw.
     rewrite H.
-    exists (match
-               app_nil_r_trans tvs in (_ = tvs')
-               return (hlist _ (tus ++ tus') -> hlist _ tvs' -> typD nil t)
-             with
-               | eq_refl => x
-             end).
-    split.
-    { clear. revert x. destruct (app_nil_r_trans tvs). reflexivity. }
-    { intros. erewrite H0.
-      instantiate (1 := Hnil).
-      instantiate (1 := us').
-      clear.
-      rewrite hlist_app_nil_r at 1.
-      revert x. revert vs. destruct (app_nil_r_trans tvs).
-      reflexivity. }
+    eexists; split; [ reflexivity | ].
+    intros. specialize (H0 us vs us' Hnil).
+    rewrite H0. rewrite hlist_app_nil_r.
+    autorewrite with eq_rw. reflexivity.
   Qed.
 
   Lemma exprD'_weakenV (EOk : ExprOk Expr_expr)
-  : forall tus tvs tvs' e t val,
-      exprD' tus tvs e t = Some val ->
+  : forall tus tvs tvs' t e val,
+      exprD' tus tvs t e = Some val ->
       exists val',
-        exprD' tus (tvs ++ tvs') e t = Some val'
+        exprD' tus (tvs ++ tvs') t (weakenV _ tvs' e) = Some val'
         /\ forall us vs vs',
              val us vs = val' us (hlist_app vs vs').
   Proof.
@@ -144,39 +251,32 @@ Section Expr.
     instantiate (1 := @eq_refl _ _).
     instantiate (1 := app_nil_r_trans _).
     simpl.
-    rewrite H.
-    exists (match
-               app_nil_r_trans tus in (_ = tus')
-               return (hlist _ tus' -> _ -> typD nil t)
-             with
-               | eq_refl => x
-             end).
-    split.
-    { clear. revert x. destruct (app_nil_r_trans tus). reflexivity. }
-    { intros. erewrite H0.
-      instantiate (1 := vs').
-      instantiate (1 := Hnil).
-      clear.
-      rewrite hlist_app_nil_r at 1.
-      revert x. revert us. destruct (app_nil_r_trans tus).
-      reflexivity. }
+    unfold weakenV.
+    autorewrite with eq_rw.
+    rewrite H. eexists; split; [ reflexivity | ].
+    intros.
+    rewrite (H0 us vs Hnil vs').
+    rewrite hlist_app_nil_r.
+    autorewrite with eq_rw.
+    reflexivity.
   Qed.
-
+(*
   Theorem exprD_weaken (EOk : ExprOk Expr_expr)
   : forall us us' vs vs' e t val,
-      exprD us vs e t = Some val ->
-      exprD (us ++ us') (vs ++ vs') e t = Some val.
+      exprD us vs t e = Some val ->
+      exprD (us ++ us') (vs ++ vs') t e = Some val.
   Proof.
     unfold exprD. intros.
     repeat rewrite split_env_app.
     destruct (split_env us); destruct (split_env us');
     destruct (split_env vs); destruct (split_env vs').
-    consider (exprD' x x1 e t); intros; try congruence.
+    consider (exprD' x x1 t e); intros; try congruence.
     inversion H0; clear H0; subst.
     eapply exprD'_weaken in H; eauto with typeclass_instances.
     destruct H. destruct H.
     rewrite H. rewrite <- H0. reflexivity.
   Qed.
+*)
 
   Lemma list_rev_ind
   : forall T (P : list T -> Prop),
@@ -190,15 +290,14 @@ Section Expr.
     simpl. auto.
   Qed.
 
-  Require Import ExtLib.Data.Eq.
-
+(*
   Theorem exprD'_strengthenU_multi (EOk : ExprOk Expr_expr)
-  : forall tus tvs e  t' tus' val,
+  : forall tus tvs e t' tus' val,
       (forall u, u < length tus' ->
                  mentionsU (length tus + u) e = false) ->
-      exprD' (tus ++ tus') tvs e t' = Some val ->
+      exprD' (tus ++ tus') tvs t' e = Some val ->
       exists val',
-        exprD' tus tvs e t' = Some val' /\
+        exprD' tus tvs t' e = Some val' /\
         forall us vs us',
           val (hlist_app us us') vs = val' us vs.
   Proof.
@@ -207,16 +306,15 @@ Section Expr.
     { simpl. intros.
       rewrite exprD'_conv with (pfu := app_nil_r_trans tus) (pfv := eq_refl).
       rewrite H0.
-      unfold ResType. rewrite eq_option_eq.
+      autorewrite with eq_rw.
       eexists; split; eauto.
       intros. rewrite (hlist_eta us').
       rewrite hlist_app_nil_r.
       clear.
-      repeat first [ rewrite eq_Const_eq | rewrite eq_Arr_eq ].
-      reflexivity. }
+      autorewrite with eq_rw. reflexivity. }
     { intros.
       rewrite exprD'_conv with (pfu := app_ass_trans tus ls (l :: nil)) (pfv := eq_refl) in H1.
-      unfold ResType in H1. rewrite eq_option_eq in H1.
+      autorewrite with eq_rw in H1.
       forward.
       eapply exprD'_strengthenU_single in H1.
       + forward_reason.
@@ -230,7 +328,7 @@ Section Expr.
                          vs (hlist_hd (snd (hlist_split _ _ us')))).
           rewrite <- H4; clear H4.
           rewrite <- H3; clear H3.
-          repeat rewrite eq_Arr_eq. repeat rewrite eq_Const_eq.
+          autorewrite with eq_rw.
           f_equal.
           rewrite hlist_app_assoc.
           apply match_eq_match_eq.
@@ -248,14 +346,13 @@ Section Expr.
         apply H0. rewrite app_length. simpl. omega. }
   Qed.
 
-
   Theorem exprD'_strengthenV_multi (EOk : ExprOk Expr_expr)
   : forall tus tvs e  t' tvs' val,
       (forall v, v < length tvs' ->
                  mentionsV (length tvs + v) e = false) ->
-      exprD' tus (tvs ++ tvs') e t' = Some val ->
+      exprD' tus (tvs ++ tvs') t' e = Some val ->
       exists val',
-        exprD' tus tvs e t' = Some val' /\
+        exprD' tus tvs t' e = Some val' /\
         forall us vs vs',
           val us (hlist_app vs vs') = val' us vs.
   Proof.
@@ -264,16 +361,16 @@ Section Expr.
     { simpl. intros.
       rewrite exprD'_conv with (pfv := app_nil_r_trans tvs) (pfu := eq_refl).
       rewrite H0.
-      unfold ResType. rewrite eq_option_eq.
+      autorewrite with eq_rw.
       eexists; split; eauto.
       intros. rewrite (hlist_eta vs').
       rewrite hlist_app_nil_r.
       clear.
-      repeat first [ rewrite eq_Const_eq | rewrite eq_Arr_eq ].
+      autorewrite with eq_rw.
       reflexivity. }
     { intros.
       rewrite exprD'_conv with (pfv := app_ass_trans tvs ls (l :: nil)) (pfu := eq_refl) in H1.
-      unfold ResType in H1. rewrite eq_option_eq in H1.
+      autorewrite with eq_rw in H1.
       forward.
       eapply exprD'_strengthenV_single in H1.
       + forward_reason.
@@ -287,14 +384,12 @@ Section Expr.
                          (hlist_hd (snd (hlist_split _ _ vs')))).
           rewrite <- H4; clear H4.
           rewrite <- H3; clear H3.
-          repeat rewrite eq_Arr_eq. repeat rewrite eq_Const_eq.
+          autorewrite with eq_rw.
           f_equal.
           rewrite hlist_app_assoc.
           apply match_eq_match_eq.
           f_equal.
-          etransitivity.
-          symmetry.
-          eapply (hlist_app_hlist_split _ _ vs').
+          rewrite <- (hlist_app_hlist_split _ _ vs') at 1.
           f_equal.
           rewrite (hlist_eta (snd (hlist_split _ _ _))).
           simpl. f_equal.
@@ -304,12 +399,12 @@ Section Expr.
       + rewrite app_length.
         apply H0. rewrite app_length. simpl. omega. }
   Qed.
-
+*)
 End Expr.
 
 Arguments Safe_expr {_ _ _ Expr} _ _ _ _ : rename.
 Arguments exprD' {_ _ _ Expr} _ _ _ _ : rename.
-Arguments exprD {_ _ _ Expr} _ _ _ _ : rename.
+(*Arguments exprD {_ _ _ Expr} _ _ _ _ : rename. *)
 Arguments ResType {_ RType} _ _ _ : rename.
-Arguments mentionsU {_ RType _ Expr} _ _ : rename.
-Arguments mentionsV {_ RType _ Expr} _ _ : rename.
+Arguments mentionsU {_ RType _ Expr} _ _ _ _ _ : rename.
+Arguments mentionsV {_ RType _ Expr} _ _ _ _ _ : rename.
