theories/InstantiateI.v
@@ -5,41 +5,55 @@ Require Import MirrorCore.ExprI.
 Require Import MirrorCore.TypesI.
 
 Section definitions.
-  Variables typ expr : Type.
+  Variables typ : Type.
+  Variable expr : tenv typ -> tenv typ -> typ -> Type.
   Context {RType_typ : RType typ}.
   Context {Expr_expr : Expr _ expr}.
   Context {ExprOk_expr : ExprOk Expr_expr}.
 
+  (** instantiate = substituteU **)
+
+  Definition subst_fn (tus tvs : tenv typ) : Type
+  := forall (n : nat) (t : typ), option (expr tus tvs t).
+
   (** instantiate **)
-  Variable instantiate : (nat -> option expr) -> nat -> expr -> expr.
+  Variable instantiate
+  : forall tus tvs t,
+      subst_fn tus tvs ->
+      forall tvs',
+      expr tus (tvs' ++ tvs) t -> expr tus (tvs' ++ tvs) t.
 
   Definition sem_preserves_if tus tvs
              (P : hlist _ tus -> hlist _ tvs -> Prop)
-             (f : nat -> option expr) : Prop :=
-    forall u e t get,
-      f u = Some e ->
+             (f : subst_fn tus tvs) : Prop :=
+    forall u t (e : expr tus tvs t) get,
+      f u t = Some e ->
       nth_error_get_hlist_nth _ tus u = Some (@existT _ _ t get) ->
       exists eD,
-        exprD' tus tvs e t = Some eD /\
+        exprD' tus tvs t e = Some eD /\
         forall us vs,
           P us vs ->
           get us = eD us vs.
 
+(*
   Definition instantiate_mentionsU : Prop :=
-    forall f n e u,
-      mentionsU u (instantiate f n e) = true <-> (** do i need iff? **)
+    forall tus tvs t f n e u,
+      mentionsU tus tvs t u (instantiate f n e) = true <-> (** do i need iff? **)
       (   (f u = None /\ mentionsU u e = true)
        \/ exists u' e',
             f u' = Some e' /\
-            mentionsU u' e = true/\
+            mentionsU u' e = true /\
             mentionsU u e' = true).
+*)
+
+  Check instantiate.
 
   Definition exprD'_instantiate : Prop :=
-    forall tus tvs f e tvs' t eD P,
+    forall tus tvs tvs' t f e eD P,
       sem_preserves_if tus tvs P f ->
-      exprD' tus (tvs' ++ tvs) e t = Some eD ->
+      exprD' tus (tvs' ++ tvs) t e = Some eD ->
       exists eD',
-        exprD' tus (tvs' ++ tvs) (instantiate f (length tvs') e) t = Some eD' /\
+        exprD' tus (tvs' ++ tvs) t (@instantiate tus tvs t f tvs' e) = Some eD' /\
         forall us vs vs',
           P us vs ->
           eD us (hlist_app vs' vs) = eD' us (hlist_app vs' vs).
